context tc

code/cs.v
@@ -19,4 +19,33 @@ Definition nat_EqType := @bEQ nat Nat.eqb nat_eqb_spec.
 
 Canonical Structure nat_EqType.
 
-Goal forall x, eqb x x = true /\ x = 3.
+Goal forall x, eqb x x = true /\ x = 3. Abort.
+
+Module mini_example.
+
+  (*SNIP: cs_struct*)
+    Structure eqType := Pack { obj : Type; eq : obj -> obj -> bool }.
+  (*ENDSNIP: cs_struct*)
+
+  Arguments eq {_}.
+  Set Printing All.
+  Check eq.
+  Fail Check (eq _ 3 3).
+
+  (*SNIP: cs*)
+    Canonical Structure eqNat : eqType := Pack nat Nat.eqb.
+  (*ENDSNIP: cs*)
+
+  Set Printing All.
+  Check (eq 3 3).
+End mini_example.
+
+Module with_class.
+  Class eqType := Pack { obj : Type; eq : obj -> obj -> bool }.
+  Set Printing All.
+  Check eq.
+  Check (eq 3 3).
+  Instance eqNat : eqType := Pack nat Nat.eqb.
+
+  Check (eq 3 3).
+End with_class.
