code/ralf.v
@@ -1,0 +1,150 @@
+(* from here: https://www.ralfj.de/blog/2019/05/15/typeclasses-exponential-blowup.html *)
+Require Import Lia ZArith.
+
+(** The operations as typeclasses for overloading, without any axioms. *)
+Class Op (A: Type) := op : A -> A -> A.
+Infix "+" := op.
+
+Class Unit (A: Type) := unit : A.
+
+Class Inverse (A: Type) := inv : A -> A.
+
+(** The algebraic classes adding the axioms, taking the operations as indices. *)
+Class Semigroup (A: Type) `{Op A} := {
+  assoc a b c : (a + b) + c = a + (b + c);
+}.
+
+Class Monoid (A: Type) `{Semigroup A, Unit A} := {
+  id_r a : a + unit = a;
+  id_l a : unit + a = a;
+}.
+
+Class Group (A: Type) `{Monoid A, Inverse A} := {
+  inv_r a : a + inv a = unit;
+  inv_l a : inv a + a = unit;
+}.
+
+
+Instance Z_op: Op Z := Z.add.
+Instance Z_unit: Unit Z := 0%Z.
+Instance Z_inv: Inverse Z := Z.opp.
+
+Instance Z_semigroup: Semigroup Z.
+Proof. split. intros. unfold op, Z_op. lia. Qed.
+Instance Z_monoid: Monoid Z.
+Proof. split; intros; unfold op, Z_op, unit, Z_unit; lia. Qed.
+Instance Z_group: Group Z.
+Proof. split; intros; unfold op, Z_op, unit, Z_unit, inv, Z_inv; lia. Qed.
+
+Section prod.
+  Context {A B: Type}.
+
+  Global Instance prod_op `{Op A, Op B}: Op (A * B) :=
+    fun '(a1, b1) '(a2, b2) => (a1 + a2, b1 + b2).
+  Global Instance prod_unit `{Unit A, Unit B}: Unit (A * B) :=
+    (unit, unit).
+  Global Instance prod_inv `{Inverse A, Inverse B}: Inverse (A * B) :=
+    fun '(a, b) => (inv a, inv b).
+
+  Global Instance prod_semigroup `{Semigroup A, Semigroup B}: Semigroup (A * B).
+  Proof.
+    split. intros [a1 b1] [a2 b2] [a3 b3]. unfold op, prod_op.
+    rewrite !assoc. reflexivity.
+  Qed.
+  Global Instance prod_monoid `{Monoid A, Monoid B}: Monoid (A * B).
+  Proof.
+    split; intros [a b]; unfold op, prod_op, unit, prod_unit;
+      rewrite ?id_l, ?id_r; reflexivity.
+  Qed.
+  Global Instance prod_group `{Group A, Group B}: Group (A * B).
+  Proof.
+    split; intros [a b]; unfold op, prod_op, unit, prod_unit, inv, prod_inv;
+      rewrite ?inv_l, ?inv_r; reflexivity.
+  Qed.
+End prod.
+
+Definition test: Group (Z*Z*Z*Z) := _.
+Set Printing All.
+Print test.
+
+(* 
+@prod_group (prod (prod Z Z) Z) Z
+  (@prod_op (prod Z Z) Z (@prod_op Z Z Z_op Z_op) Z_op)
+  (@prod_semigroup (prod Z Z) Z (@prod_op Z Z Z_op Z_op)
+	 (@prod_semigroup Z Z Z_op Z_semigroup Z_op Z_semigroup) Z_op Z_semigroup)
+  (@prod_unit (prod Z Z) Z (@prod_unit Z Z Z_unit Z_unit) Z_unit)
+  (@prod_monoid (prod Z Z) Z (@prod_op Z Z Z_op Z_op)
+     (@prod_semigroup Z Z Z_op Z_semigroup Z_op Z_semigroup)
+     (@prod_unit Z Z Z_unit Z_unit)
+     (@prod_monoid Z Z Z_op Z_semigroup Z_unit Z_monoid Z_op Z_semigroup
+        Z_unit Z_monoid)
+     Z_op Z_semigroup Z_unit Z_monoid)
+  (@prod_inv (prod Z Z) Z (@prod_inv Z Z Z_inv Z_inv) Z_inv)
+  (@prod_group (prod Z Z) Z (@prod_op Z Z Z_op Z_op)
+     (@prod_semigroup Z Z Z_op Z_semigroup Z_op Z_semigroup)
+     (@prod_unit Z Z Z_unit Z_unit)
+     (@prod_monoid Z Z Z_op Z_semigroup Z_unit Z_monoid Z_op Z_semigroup
+        Z_unit Z_monoid)
+     (@prod_inv Z Z Z_inv Z_inv)
+     (@prod_group Z Z Z_op Z_semigroup Z_unit Z_monoid Z_inv Z_group Z_op
+        Z_semigroup Z_unit Z_monoid Z_inv Z_group)
+     Z_op Z_semigroup Z_unit Z_monoid Z_inv Z_group)
+  Z_op Z_semigroup Z_unit Z_monoid Z_inv Z_group
+     : @Group (prod (prod (prod Z Z) Z) Z)
+         (@prod_op (prod (prod Z Z) Z) Z
+            (@prod_op (prod Z Z) Z (@prod_op Z Z Z_op Z_op) Z_op) Z_op)
+         (@prod_semigroup (prod (prod Z Z) Z) Z
+            (@prod_op (prod Z Z) Z (@prod_op Z Z Z_op Z_op) Z_op)
+            (@prod_semigroup (prod Z Z) Z (@prod_op Z Z Z_op Z_op)
+               (@prod_semigroup Z Z Z_op Z_semigroup Z_op Z_semigroup) Z_op
+               Z_semigroup)
+            Z_op Z_semigroup)
+         (@prod_unit (prod (prod Z Z) Z) Z
+            (@prod_unit (prod Z Z) Z (@prod_unit Z Z Z_unit Z_unit) Z_unit)
+            Z_unit)
+         (@prod_monoid (prod (prod Z Z) Z) Z
+            (@prod_op (prod Z Z) Z (@prod_op Z Z Z_op Z_op) Z_op)
+            (@prod_semigroup (prod Z Z) Z (@prod_op Z Z Z_op Z_op)
+               (@prod_semigroup Z Z Z_op Z_semigroup Z_op Z_semigroup) Z_op
+               Z_semigroup)
+            (@prod_unit (prod Z Z) Z (@prod_unit Z Z Z_unit Z_unit) Z_unit)
+            (@prod_monoid (prod Z Z) Z (@prod_op Z Z Z_op Z_op)
+               (@prod_semigroup Z Z Z_op Z_semigroup Z_op Z_semigroup)
+               (@prod_unit Z Z Z_unit Z_unit)
+               (@prod_monoid Z Z Z_op Z_semigroup Z_unit Z_monoid Z_op
+                  Z_semigroup Z_unit Z_monoid)
+               Z_op Z_semigroup Z_unit Z_monoid)
+            Z_op Z_semigroup Z_unit Z_monoid)
+         (@prod_inv (prod (prod Z Z) Z) Z
+            (@prod_inv (prod Z Z) Z (@prod_inv Z Z Z_inv Z_inv) Z_inv) Z_inv)
+*)
+
+(* 
+let p0 := prod Z Z in
+let p1 := prod p0 Z in
+let xx := (@prod_op Z Z Z_op Z_op) in
+let aa := @prod_op p0 Z xx Z_op in
+
+let bb := @prod_semigroup Z Z Z_op Z_semigroup Z_op Z_semigroup in
+let cc := @prod_semigroup p0 Z xx bb Z_op Z_semigroup in
+
+let pu1 := prod_unit Z Z Z_unit Z_unit in
+let pu2 := @prod_unit p0 Z pu1 Z_unit in
+
+let pp01 := prod_monoid Z Z Z_op Z_semigroup Z_unit Z_monoid Z_op Z_semigroup Z_unit Z_monoid in
+let pm2 := prod_monoid p0 Z xx bb pu1 pp01 Z_op Z_semigroup Z_unit Z_monoid in
+let piv := @prod_inv Z Z Z_inv Z_inv) in
+let piv2 := prod_inv p0 Z pi0 Z_inv in
+
+@prod_group p1 Z aa cc pu2 pm2 piv2
+  (@prod_group p0 Z xx bb pu1 pp01 pi0
+     (@prod_group Z Z Z_op Z_semigroup Z_unit Z_monoid Z_inv Z_group Z_op Z_semigroup Z_unit Z_monoid Z_inv Z_group)
+     Z_op Z_semigroup Z_unit Z_monoid Z_inv Z_group)
+  Z_op Z_semigroup Z_unit Z_monoid Z_inv Z_group
+     : @Group (prod p1 Z)
+         (@prod_op p1 Z aa Z_op)
+         (@prod_semigroup p1 Z aa cc Z_op Z_semigroup)
+         (@prod_unit p1 Z pu2 Z_unit)
+         (@prod_monoid p1 Z aa cc pu2 pm2 Z_op Z_semigroup Z_unit Z_monoid)
+         (@prod_inv p1 Z piv2 Z_inv)
+*)
